Enabling portfolio mode

Examples/Set.lean
@@ -6,8 +6,14 @@ These are adapted from Mathematics in Lean. The relevant definitions are in the 
 -/
 import Mathlib.Data.Nat.Prime
 import Mathlib.Data.Set.Lattice
+import Auto.Tactic
 
 open Set
+
+set_option trace.auto.tptp.printQuery true
+set_option trace.auto.tptp.result true
+set_option tptp.solver.name "zeport"
+set_option tptp.zeport.path "/home/indprinciple/Programs/zipperposition/portfolio/portfolio.fo.parallel.py"
 
 variable {α β : Type _}
 
@@ -19,34 +25,39 @@ variable (s t u : Set α)
 #check mem_union
 #check Set.ext
 
+-- Blocking duper so that examples run faster
+-- Duper succeeds on one of the following examples
+set_option maxHeartbeats 5000
+
 example (h : s ⊆ t) : s ∩ u ⊆ t ∩ u := by
-  sorry
+  auto [mem_inter_iff, subset_def, h]
 
 example : s ∩ (t ∪ u) ⊆ s ∩ t ∪ s ∩ u := by
-  sorry
+  auto [mem_inter_iff, mem_union, subset_def]
 
 example : s ∩ t ∪ s ∩ u ⊆ s ∩ (t ∪ u) := by
-  sorry
+  auto [mem_inter_iff, mem_union, subset_def]
 
 #check mem_diff
 
 example : (s \ t) \ u ⊆ s \ (t ∪ u) := by
-  sorry
+  auto [mem_diff, mem_union, subset_def]
 
 example : s ∩ t = t ∩ s := by
-  sorry
+  auto [Set.ext, mem_inter_iff]
 
 example : s ∩ (s ∪ t) = s := by
-  sorry
+  auto [Set.ext, mem_union, mem_inter_iff]
 
 example : s ∪ s ∩ t = s := by
-  sorry
+  auto [Set.ext, mem_union, mem_inter_iff]
 
+set_option maxHeartbeats 200000 in
 example : s \ t ∪ t = s ∪ t := by
-  sorry
+  apply Set.ext; auto [mem_union, mem_diff]
 
 example : s \ t ∪ t \ s = (s ∪ t) \ (s ∩ t) := by
-  sorry
+  apply Set.ext; auto [mem_union, mem_inter_iff, mem_diff]
 
 #check mem_setOf
 
@@ -56,17 +67,20 @@ def evens : Set ℕ :=
 def odds : Set ℕ :=
   { n | ¬Even n }
 
+set_option auto.prep.redMode "all" in
 example : evens ∪ odds = univ := by
-  sorry
+  auto
 
 #check mem_empty_iff_false
 #check mem_univ
 
-example (x : ℕ) (h : x ∈ (∅ : Set ℕ)) : False :=
-  sorry
+set_option auto.prep.redMode "all" in
+example (x : ℕ) (h : x ∈ (∅ : Set ℕ)) : False := by
+  auto
 
-example (x : ℕ) : x ∈ (univ : Set ℕ) :=
-  trivial
+set_option auto.prep.redMode "all" in
+example (x : ℕ) : x ∈ (univ : Set ℕ) := by
+  auto
 
 example : { n | Nat.Prime n } ∩ { n | n > 2 } ⊆ { n | ¬Even n } := by
   sorry
@@ -77,19 +91,19 @@ section
 variable (s t : Set ℕ)
 
 example (h₀ : ∀ x ∈ s, ¬Even x) (h₁ : ∀ x ∈ s, Prime x) : ∀ x ∈ s, ¬Even x ∧ Prime x := by
-  sorry
+  auto [h₀, h₁]
 
 example (h : ∃ x ∈ s, ¬Even x ∧ Prime x) : ∃ x ∈ s, Prime x := by
-  sorry
+  auto [h]
 
 section
 variable (ssubt : s ⊆ t)
 
 example (h₀ : ∀ x ∈ t, ¬Even x) (h₁ : ∀ x ∈ t, Prime x) : ∀ x ∈ s, ¬Even x ∧ Prime x := by
-  sorry
+  auto [h₀, h₁, ssubt, subset_def]
 
 example (h : ∃ x ∈ s, ¬Even x ∧ Prime x) : ∃ x ∈ t, Prime x := by
-  sorry
+  auto [h, ssubt, subset_def]
 
 end
 
@@ -106,28 +120,31 @@ open Set
 #check mem_iInter
 
 example : (s ∩ ⋃ i, A i) = ⋃ i, A i ∩ s := by
-  sorry
+  apply Set.ext; auto [mem_inter_iff, mem_iUnion]
 
 example : (⋂ i, A i ∩ B i) = (⋂ i, A i) ∩ ⋂ i, B i := by
-  sorry
+  apply Set.ext; auto [mem_inter_iff, mem_iInter]
 
 example : (s ∪ ⋂ i, A i) = ⋂ i, A i ∪ s := by
-  sorry
+  apply Set.ext; auto [mem_union, mem_iInter]
 
-def primes : Set ℕ :=
+def primeset : Set ℕ :=
   { x | Nat.Prime x }
 
-example : (⋃ p ∈ primes, { x | p ^ 2 ∣ x }) = { x | ∃ p ∈ primes, p ^ 2 ∣ x } :=by
-  sorry
+set_option trace.auto.lamReif.printResult true in
+example : (⋃ p ∈ primeset, { x | p ^ 2 ∣ x }) = { x | ∃ p ∈ primeset, p ^ 2 ∣ x } := by
+  apply Set.ext; intro x
+  rw [mem_iUnion]; conv => enter [1, 1, i]; rw [mem_iUnion]
+  simp
 
 #check Nat.exists_prime_and_dvd
 
-example : (⋂ p ∈ primes, { x | ¬p ∣ x }) ⊆ { x | x = 1 } := by
+example : (⋂ p ∈ primeset, { x | ¬p ∣ x }) ⊆ { x | x = 1 } := by
   sorry
 
 #check Nat.exists_infinite_primes
 
-example : (⋃ p ∈ primes, { x | x ≤ p }) = univ := by
+example : (⋃ p ∈ primeset, { x | x ≤ p }) = univ := by
   sorry
 
 end
@@ -140,6 +157,9 @@ variable {α : Type _} (s : Set (Set α))
 #check mem_iUnion₂
 #check mem_iInter₂
 
+set_option trace.auto.tptp.printQuery true
+set_option trace.auto.tptp.result true
+
 example : ⋃₀ s = ⋃ t ∈ s, t := by
   sorry
 
@@ -147,4 +167,3 @@ example : ⋂₀ s = ⋂ t ∈ s, t := by
   sorry
 
 end
-
