Auto/Solver/TPTP.lean
@@ -54,18 +54,30 @@ def queryZipperposition (query : String) : MetaM Unit := do
 
 def queryZEPort (query : String) : MetaM Unit := do
   let path := tptp.zeport.path.get (← getOptions)
-  if !(← System.FilePath.pathExists ".zeport_ignore") then
-    IO.FS.createDir "./.zeport_ignore"
-  let idx ← IO.monoMsNow
+  -- To avoid concurrency issue, use `attempt`
+  attempt <| IO.FS.createDir "./.zeport_ignore"
+  let mut idx := 0
+  -- Synchronization
+  while true do
+    try
+      IO.FS.createDir s!"./.zeport_ignore/tmp{idx}"
+      break
+    catch e =>
+      let estr := toString (← (Exception.toMessageData e).format)
+      if estr.extract ⟨0⟩ ⟨44⟩ != "already exists (error code: 17, file exists)" then
+        throwError "queryZEPort :: Unexpected error"
+      idx := idx + (← IO.rand 0 100)
   IO.FS.withFile s!"./.zeport_ignore/problem{idx}.p" .writeNew (fun stream =>
     stream.putStr query)
-  IO.FS.createDir s!"./.zeport_ignore/tmp{idx}"
-  let solver ← createAux path #[s!"./.zeport_ignore/problem{idx}.p", "10", s!"./.zeport_ignore/tmp{idx}"]
-  let result ← solver.stdout.readToEnd
-  trace[auto.tptp.result] "Result: {result}"
+  let solver ← createAux "python3" #[path, s!"./.zeport_ignore/problem{idx}.p", "10", s!"./.zeport_ignore/tmp{idx}"]
+  let stderr ← solver.stderr.readToEnd
+  let stdout ← solver.stdout.readToEnd
+  trace[auto.tptp.result] "Result: \nstderr: {stderr}\nstdout: {stdout}"
   solver.kill
-  -- IO.FS.removeFile s!"./.zeport_ignore/problem{idx}.p"
+  IO.FS.removeFile s!"./.zeport_ignore/problem{idx}.p"
+  -- For synchronization, remove directory in the end
   IO.FS.removeDir s!"./.zeport_ignore/tmp{idx}"
+where attempt (action : MetaM Unit) := try action catch _ => pure ()
 
 def querySolver (query : String) : MetaM Unit := do
   match tptp.solver.name.get (← getOptions) with
