Test/Test_regression.lean
@@ -4,6 +4,11 @@ set_option auto.prep.redMode "reducible"
 set_option trace.auto.lamReif.printResult true
 set_option trace.auto.lamReif.printValuation true
 
+-- set_option trace.auto.tptp.printQuery true
+-- set_option trace.auto.tptp.result true
+-- set_option tptp.solver.name "zeport"
+-- set_option tptp.zeport.path "/home/indprinciple/Programs/zipperposition/portfolio/portfolio.fo.parallel.py"
+
 -- Manual Check
 
 section ManualCheck
